Added the definition model_eval, which checks if a thing is true in every world.

BML/Def.lean
@@ -49,6 +49,14 @@ def eval {World Atom} (M : Model World Atom) (w : World) : Proposition Atom → 
   | .and φ1 φ2 => eval M w φ1 ∧ eval M w φ2
   | .diamond φ => ∃ x : World, M.r w x ∧ eval M x φ
 
+/-- M ⊨ φ -/
+def model_eval {World Atom} (M : Model World Atom) : Proposition Atom → Prop
+  | φ => ∀ w : World, eval M w φ
+
+/-- M ⊨ φ iff for all world w: M ⊨ φ -/
+lemma model_true {World Atom} (M : Model World Atom) (φ : Proposition Atom) : model_eval M φ ↔ ∀w : World, eval M w φ := by
+  trivial
+
 def Proposition.or : Proposition A → Proposition A → Proposition A
   | φ1, φ2 => (φ1.not.and φ2.not).not
 
